DinD: Use error monad in translator
This is needed because we want to report the source of translation issues, but
we can't store C# AST objects into !new expressions.  The downside is that we
get errors one at a time.

Source/DafnyCompilers/CSharpDafnyInterop.cs
@@ -33,5 +33,8 @@ namespace CSharpDafnyInterop {
 
     public static BigInteger Numerator(Dafny.BigRational r) => r.num;
     public static BigInteger Denominator(Dafny.BigRational r) => r.den;
+
+    public static Dafny.ISequence<char> ObjectToString(object o) =>
+      AsString((o ?? "null").ToString());
   }
 }
